theories/DSub/typing/ds_storeless_typing.v
@@ -31,7 +31,7 @@ Inductive typed Γ : tm → ty → Prop :=
     (* After looking up in Γ, we must weaken T for the variables on top of x. *)
     Γ !! x = Some T →
     (*──────────────────────*)
-    Γ ⊢ₜ tv (var_vl x) : shiftN x T
+    Γ ⊢ₜ tv (vvar x) : shiftN x T
 | iT_ISub e T1 T2 i :
     Γ ⊢ₜ T1, 0 <: T2, i → Γ ⊢ₜ e : T1 →
     (*───────────────────────────────*)
