theories/Dot/examples/old_typing/old_subtyping.v
@@ -15,7 +15,7 @@ Inductive path_typed Γ : path → ty → nat → Prop :=
 | iP_Var x T:
     Γ !! x = Some T →
     (* After looking up in Γ, we must weaken T for the variables on top of x. *)
-    Γ u⊢ₚ pv (var_vl x) : shiftN x T, 0
+    Γ u⊢ₚ pv (vvar x) : shiftN x T, 0
 | iP_Nat_I n:
     Γ u⊢ₚ pv (vint n): TInt, 0
 | iP_Bool_I b:
@@ -221,13 +221,13 @@ Lemma iP_Var' Γ x T1 T2 :
   Γ !! x = Some T1 →
   T2 = shiftN x T1 →
   (*──────────────────────*)
-  Γ u⊢ₚ pv (var_vl x) : T2, 0.
+  Γ u⊢ₚ pv (vvar x) : T2, 0.
 Proof. by intros; subst; constructor. Qed.
 
 Lemma iP_Var0 Γ T :
   Γ !! 0 = Some T →
   (*──────────────────────*)
-  Γ u⊢ₚ pv (var_vl 0) : T, 0.
+  Γ u⊢ₚ pv (vvar 0) : T, 0.
 Proof. intros; eapply iP_Var'; by rewrite ?hsubst_id. Qed.
 
 Ltac pvar := exact: iP_Var0 || exact: iP_Var'.
@@ -236,29 +236,29 @@ Lemma iP_Var_Sub Γ x T1 T2 :
   Γ !! x = Some T1 →
   Γ u⊢ₜ shiftN x T1, 0 <: T2, 0 →
   (*──────────────────────*)
-  Γ u⊢ₚ pv (var_vl x) : T2, 0.
+  Γ u⊢ₚ pv (vvar x) : T2, 0.
 Proof. by intros; eapply iP_ISub'; [|pvar]. Qed.
 
 Lemma iP_Var0_Sub Γ T1 T2 :
   Γ !! 0 = Some T1 →
   Γ u⊢ₜ T1, 0 <: T2, 0 →
   (*──────────────────────*)
-  Γ u⊢ₚ pv (var_vl 0) : T2, 0.
+  Γ u⊢ₚ pv (vvar 0) : T2, 0.
 Proof. intros. by eapply iP_Var_Sub; [| rewrite ?hsubst_id]. Qed.
 
 Ltac pvarsub := (eapply iP_Var0_Sub || eapply iP_Var_Sub); first done.
 
 Lemma iP_Mu_I' x T {Γ i} :
   is_unstamped_ty' (length Γ).+1 T →
-  Γ u⊢ₚ pv (var_vl x) : T.|[ var_vl x /], i →
-  Γ u⊢ₚ pv (var_vl x) : TMu T, i.
+  Γ u⊢ₚ pv (vvar x) : T.|[ vvar x /], i →
+  Γ u⊢ₚ pv (vvar x) : TMu T, i.
 Proof.
   intros Hu Hp. by eapply iP_Mu_I; last rewrite (psubst_subst_agree_ty _ Hu).
 Qed.
 Lemma iP_Mu_E' x T {Γ i} :
   is_unstamped_ty' (length Γ).+1 T →
-  Γ u⊢ₚ pv (var_vl x) : TMu T, i →
-  Γ u⊢ₚ pv (var_vl x) : T.|[ var_vl x /], i.
+  Γ u⊢ₚ pv (vvar x) : TMu T, i →
+  Γ u⊢ₚ pv (vvar x) : T.|[ vvar x /], i.
 Proof. intros Hu Hp; rewrite -(psubst_subst_agree_ty _ Hu); exact: iP_Mu_E. Qed.
 
 Ltac typconstructor_blacklist Γ :=
